update receive invariant to avoid existential quantifier

messageInvariantPrototypes/ringLeaderElection/automate/distributedSystem.dfy
@@ -149,13 +149,13 @@ module DistributedSystem {
     Next(c, v.Truncate(c, i), v.Truncate(c, i+1))
   }
 
-  ghost predicate IsReceiveStepByActor(c: Constants, v: Variables, i:int, actor: int)
+  ghost predicate IsReceiveStepByActor(c: Constants, v: Variables, i:int, actor: int, msg: Message)
     requires v.WF(c)
     requires 1 <= i < |v.history|
     requires Next(c, v.Truncate(c, i), v.Truncate(c, i+1))
   {
     var step :| NextStep(c, v.Truncate(c, i).Last(), v.Truncate(c, i+1).Last(), v.network, v.network, step);
-    && step.msgOps.recv.Some?
+    && step.msgOps.recv == Some(msg)
     && step.actorIdx == actor
   }
 
